\documentclass{article}
\usepackage{ids}
\usepackage{planetmath-specials}
\usepackage{pmath}
\usepackage{amssymb}
\usepackage{amsmath}
\usepackage{amsfonts}
\usepackage{graphicx}
\usepackage{xypic}
\begin{document}
If $(\sigma, \delta)$ is a skew derivation on a ring $R$,
then a {\it $(\sigma, \delta)$-constant} is an element $q$ of $R$
such that $\sigma(q)=q$ and $\delta(q)=0$.
\par
Note: If $q$ is a $(\sigma, \delta)$-constant,
then it follows that $\sigma(q \cdot x)=q \cdot \sigma(x)$
and $\delta(q \cdot x)=q \cdot \delta(x)$ for all $x$ in $R$.
\end{document}
